rt spec+proof: add sporadic implies active invariant
This adds an invariant to active_scs_valid (part of valid_sched) which
states that every scheduling context which is sporadic is active.

Several changes to the specs were made, in particular

 - a sched context is made not sporadic during the finalisation process.
   This was required to prove the invariant holds.

 - the update to the sc_sporadic field within
   invoke_sched_control_configure_flags is now made towards the end of
   the function, so as to ensure that the field is updated only after the
   scheduling context is made active. This means that the new invariant is
   not broken temporarily, and eases the proofs. In addition, the update
   to the sc_badge field is moved.

 - if_cond_refill_unblock_check is modified, taking into account the
   new invariant.

Signed-off-by: Michael McInerney <michael.mcinerney@proofcraft.systems>

proof/invariant-abstract/DetSchedInvs_AI.thy
@@ -755,6 +755,7 @@ record sc_refill_cfg =
   scrc_refill_max :: nat
   scrc_period :: ticks
   scrc_budget :: ticks
+  scrc_sporadic :: bool
 
 abbreviation
   "scrc_refill_hd scrc \<equiv> hd (scrc_refills scrc)"
@@ -763,7 +764,8 @@ definition sc_refill_cfg_of :: "sched_context \<Rightarrow> sc_refill_cfg" where
   "sc_refill_cfg_of sc = \<lparr> scrc_refills = sc_refills sc,
                            scrc_refill_max = sc_refill_max sc,
                            scrc_period = sc_period sc,
-                           scrc_budget = sc_budget sc\<rparr>"
+                           scrc_budget = sc_budget sc,
+                           scrc_sporadic = sc_sporadic sc\<rparr>"
 
 definition sc_refill_cfgs_of_scs :: "('obj_ref \<rightharpoonup> sched_context) \<Rightarrow> 'obj_ref \<rightharpoonup> sc_refill_cfg" where
   "sc_refill_cfgs_of_scs \<equiv> map_project sc_refill_cfg_of"
@@ -781,6 +783,7 @@ lemma sc_refill_cfg_of_simps[iff]:
   "scrc_period (sc_refill_cfg_of sc) = sc_period sc"
   "scrc_refill_hd (sc_refill_cfg_of sc) = refill_hd sc"
   "scrc_budget (sc_refill_cfg_of sc) = sc_budget sc"
+  "scrc_sporadic (sc_refill_cfg_of sc) = sc_sporadic sc"
   by (auto simp: sc_refill_cfg_of_def)
 
 \<comment> \<open>These might not be necessary, since they're already solved by auto\<close>
@@ -792,7 +795,6 @@ lemma sc_refill_cfg_of_updates[iff]:
   "\<And>f. sc_refill_cfg_of (sc_refills_update f sc) = scrc_refills_update f (sc_refill_cfg_of sc)"
   "\<And>f. sc_refill_cfg_of (sc_refill_max_update f sc) = scrc_refill_max_update f (sc_refill_cfg_of sc)"
   "\<And>f. sc_refill_cfg_of (sc_badge_update f sc) = sc_refill_cfg_of sc"
-  "\<And>f. sc_refill_cfg_of (sc_sporadic_update f sc) = sc_refill_cfg_of sc"
   "\<And>f. sc_refill_cfg_of (sc_yield_from_update f sc) = sc_refill_cfg_of sc"
   "\<And>f. sc_refill_cfg_of (sc_replies_update f sc) = sc_refill_cfg_of sc"
   by auto
@@ -2343,7 +2345,9 @@ definition active_scs_valid_2 :: "(obj_ref \<rightharpoonup> sc_refill_cfg) \<Ri
           \<longrightarrow> pred_map cfg_valid_refills sc_refill_cfgs scp
               \<and> pred_map cfg_bounded_release_time sc_refill_cfgs scp)
    \<and> (\<forall>scp. pred_map (\<lambda>cfg. \<not> active_scrc cfg) sc_refill_cfgs scp
-            \<longrightarrow> pred_map (\<lambda>cfg. scrc_budget cfg = 0) sc_refill_cfgs scp)"
+            \<longrightarrow> pred_map (\<lambda>cfg. scrc_budget cfg = 0) sc_refill_cfgs scp)
+   \<and> (\<forall>scp. pred_map (\<lambda>cfg. scrc_sporadic cfg) sc_refill_cfgs scp
+            \<longrightarrow> pred_map (\<lambda>cfg. active_scrc cfg) sc_refill_cfgs scp)"
 
 abbreviation active_scs_valid :: "'z state \<Rightarrow> bool" where
   "active_scs_valid s \<equiv> active_scs_valid_2 (sc_refill_cfgs_of s)"
@@ -2351,14 +2355,15 @@ abbreviation active_scs_valid :: "'z state \<Rightarrow> bool" where
 lemmas active_scs_valid_def = active_scs_valid_2_def
 
 lemma active_scs_valid_lift_pre_conj:
-  assumes a: "\<And>scp. \<lbrace>\<lambda>s. \<not> pred_map active_scrc (sc_refill_cfgs_of s) scp \<and> R s\<rbrace>
-                     f \<lbrace>\<lambda>rv s. \<not> pred_map active_scrc (sc_refill_cfgs_of s) scp\<rbrace>"
+  assumes a:
+    "\<And>scp P Q. \<lbrace>\<lambda>s. Q (pred_map (\<lambda>cfg. P (active_scrc cfg)) (sc_refill_cfgs_of s) scp) \<and> R s\<rbrace>
+                f \<lbrace>\<lambda>rv s. Q (pred_map (\<lambda>cfg. P (active_scrc cfg)) (sc_refill_cfgs_of s) scp)\<rbrace>"
   assumes b: "\<And>scp. \<lbrace>\<lambda>s. valid_refills scp s \<and> R s\<rbrace> f \<lbrace>\<lambda>rv s. valid_refills scp s\<rbrace>"
   assumes c: "\<And>scp. \<lbrace>\<lambda>s. bounded_release_time scp s \<and> R s\<rbrace> f \<lbrace>\<lambda>rv s. bounded_release_time scp s\<rbrace>"
-  assumes d: "\<And>scp. \<lbrace>\<lambda>s. \<not> pred_map (\<lambda>cfg. \<not> active_scrc cfg) (sc_refill_cfgs_of s) scp \<and> R s\<rbrace>
-                     f \<lbrace>\<lambda>rv s. \<not> pred_map (\<lambda>cfg. \<not> active_scrc cfg) (sc_refill_cfgs_of s) scp\<rbrace>"
-  assumes e: "\<And>scp. \<lbrace>\<lambda>s. pred_map (\<lambda>cfg. scrc_budget cfg = 0) (sc_refill_cfgs_of s) scp \<and> R s\<rbrace>
+  assumes d: "\<And>scp. \<lbrace>\<lambda>s. pred_map (\<lambda>cfg. scrc_budget cfg = 0) (sc_refill_cfgs_of s) scp \<and> R s\<rbrace>
                      f \<lbrace>\<lambda>_ s. pred_map (\<lambda>cfg. scrc_budget cfg = 0) (sc_refill_cfgs_of s) scp\<rbrace>"
+  assumes e: "\<And>scp. \<lbrace>\<lambda>s. \<not> pred_map (\<lambda>cfg. scrc_sporadic cfg) (sc_refill_cfgs_of s) scp \<and> R s\<rbrace>
+                     f \<lbrace>\<lambda>_ s. \<not> pred_map (\<lambda>cfg. scrc_sporadic cfg) (sc_refill_cfgs_of s) scp\<rbrace>"
     shows "\<lbrace>\<lambda>s. active_scs_valid s \<and> R s\<rbrace> f \<lbrace>\<lambda>rv. active_scs_valid\<rbrace>"
   apply (simp add: active_scs_valid_def)
   apply (wpsimp wp: hoare_vcg_all_lift hoare_vcg_imp_lift' a b c d e)
@@ -3552,12 +3557,14 @@ lemma active_reply_scs_lift_pre_conj:
 lemma valid_sched_lift_pre_conj:
   assumes "\<And>N P t. \<lbrace>\<lambda>s. N (pred_map P (tcb_sts_of s) t) \<and> R s\<rbrace> f \<lbrace>\<lambda>rv s. N (pred_map P (tcb_sts_of s) t)\<rbrace>"
   assumes "\<And>P t. \<lbrace>\<lambda>s. P (active_sc_tcb_at t s) \<and> R s\<rbrace> f \<lbrace>\<lambda>rv s. P (active_sc_tcb_at t s)\<rbrace>"
-  assumes "\<And>t. \<lbrace>\<lambda>s. \<not> pred_map active_scrc (sc_refill_cfgs_of s) t \<and> R s\<rbrace>
-               f \<lbrace>\<lambda>rv s. \<not> pred_map active_scrc (sc_refill_cfgs_of s) t\<rbrace>"
+  assumes "\<And>P Q t. \<lbrace>\<lambda>s. Q (pred_map (\<lambda>cfg. P (active_scrc cfg)) (sc_refill_cfgs_of s) t) \<and> R s\<rbrace>
+                    f \<lbrace>\<lambda>rv s. Q (pred_map (\<lambda>cfg. P (active_scrc cfg)) (sc_refill_cfgs_of s) t)\<rbrace>"
   assumes "\<And>scp. \<lbrace>\<lambda>s. \<not> pred_map (\<lambda>cfg. \<not> active_scrc cfg) (sc_refill_cfgs_of s) scp \<and> R s\<rbrace>
                   f \<lbrace>\<lambda>_ s. \<not> pred_map (\<lambda>cfg. \<not> active_scrc cfg) (sc_refill_cfgs_of s) scp\<rbrace>"
   assumes "\<And>scp. \<lbrace>\<lambda>s. pred_map (\<lambda>cfg. scrc_budget cfg = 0) (sc_refill_cfgs_of s) scp \<and> R s\<rbrace>
                   f \<lbrace>\<lambda>_ s. pred_map (\<lambda>cfg. scrc_budget cfg = 0) (sc_refill_cfgs_of s) scp\<rbrace>"
+  assumes "\<And>scp. \<lbrace>\<lambda>s. \<not> pred_map (\<lambda>cfg. scrc_sporadic cfg) (sc_refill_cfgs_of s) scp \<and> R s\<rbrace>
+                  f \<lbrace>\<lambda>_ s. \<not> pred_map (\<lambda>cfg. scrc_sporadic cfg) (sc_refill_cfgs_of s) scp\<rbrace>"
   assumes "\<And>t. \<lbrace>\<lambda>s. valid_refills t s \<and> R s\<rbrace> f \<lbrace>\<lambda>rv s. valid_refills t s\<rbrace>"
   assumes "\<And>scp. \<lbrace>\<lambda>s. bounded_release_time scp s \<and> R s\<rbrace> f \<lbrace>\<lambda>rv s. bounded_release_time scp s\<rbrace>"
   assumes "\<And>t. \<lbrace>\<lambda>s. budget_ready t s \<and> R s\<rbrace> f \<lbrace>\<lambda>rv s. budget_ready t s\<rbrace>"
